cdemo/Demoproof.v
@@ -1,0 +1,21 @@
+Require Import Coqlib Errors.
+Require Import AST Linking Smallstep Invariant CallconvAlgebra.
+
+Require Import Conventions Mach.
+Require Import Locations.
+Require Import LanguageInterface.
+
+Require Import Integers.
+Require Import Values Memory.
+
+Require Import CallconvBig InjectFootprint Injp.
+Require Import CAnew.
+Require Import Asm Asmrel.
+Require Import Asmgenproof0 Asmgenproof1.
+Require Import Encrypt EncryptSpec Encryptproof.
+Require Import Client Server.
+
+Import GS.
+
+(** 1st step : module linking *)
+               
