concur/Asmselfsim.v
@@ -1,0 +1,248 @@
+Require Import Coqlib Mapsrel.
+Require Import AST Integers Valuesrel Eventsrel CKLR LanguageInterface Smallstep.
+Require Import Op Registersrel.
+Require Export Asm.
+
+Require Import CallConv CallconvBig Injp.
+Require Import CallconvBig InjectFootprint Injp Extends Ext.
+
+(** ext *)
+Section EXT.
+
+Variable prog: program.
+Variable w: ext_world.
+Variable se: Genv.symtbl.
+Let m10 := match w with extw m1 _ _ => m1 end.
+Let init_sup := Mem.support m10.
+Let ge := Genv.globalenv se prog.
+
+Definition regset_lessdef (rs1 rs2: regset) := forall r, Val.lessdef (rs1 r) (rs2 r).
+
+Inductive match_states : ext_world -> state -> state -> Prop :=
+|match_states_normal:
+  forall rs m rs' m' wp Hm flag
+    (RLD: regset_lessdef rs rs')
+    (ACI: ext_acci wp (extw m m' Hm))
+    (ACE: ext_acce w (extw m m' Hm)),
+  match_states wp (State rs m flag)
+               (State rs' m' flag).
+(*
+Lemma ros_address_lessdef:
+  forall ros rs rs',
+  regset_lessdef rs rs' ->
+  Val.lessdef (ros_address ge ros rs) (ros_address ge ros rs').
+Proof.
+  intros. unfold ros_address, Genv.find_funct. destruct ros; auto.
+Qed.
+
+Lemma find_funct_lessdef: forall vf vf' fd,
+    Genv.find_funct ge vf = Some fd ->
+    Val.lessdef vf vf' ->
+    Genv.find_funct ge vf' = Some fd.
+Proof.
+  intros. unfold Genv.find_funct in *. inv H0; simpl in *; try congruence.
+Qed.
+
+Lemma regs_lessdef_init_regs:
+  forall params vl vl',
+  Val.lessdef_list vl vl' ->
+  regs_lessdef (init_regs vl params) (init_regs vl' params).
+Proof.
+  induction params; intros.
+  simpl. red; intros. rewrite Regmap.gi. constructor.
+  simpl. inv H.   red; intros. rewrite Regmap.gi. constructor.
+  apply set_reg_lessdef. auto. auto.
+Qed.
+ *)
+
+Lemma regset_lessdef_set : forall rs1 rs2 r v1 v2,
+    regset_lessdef rs1 rs2 ->
+    Val.lessdef v1 v2 ->
+    regset_lessdef (rs1 # r <- v1) (rs2 # r <- v2).
+Proof.
+  intros. red. intros.
+  destruct (Pregmap.elt_eq r r0). subst.
+  rewrite !Pregmap.gss. eauto.
+  rewrite !Pregmap.gso; try congruence. eauto.
+Qed.
+
+Lemma regset_lessdef_nextinstr : forall rs1 rs2,
+    regset_lessdef rs1 rs2 ->
+    regset_lessdef (nextinstr rs1) (nextinstr rs2).
+Proof.
+  intros. unfold nextinstr.
+  eapply regset_lessdef_set; eauto.
+  generalize (H PC). intro.
+  inv H0; constructor.
+Qed.
+
+Lemma regset_lessdef_undef_regs : forall l rs1 rs2,
+    regset_lessdef rs1 rs2 ->
+    regset_lessdef (undef_regs l rs1) (undef_regs l rs2).
+Proof.
+  induction l; intros; simpl; eauto.
+  eapply IHl.
+  eapply regset_lessdef_set; eauto.
+Qed.
+  
+Lemma regset_lessdef_nextinstr_nf : forall rs1 rs2,
+    regset_lessdef rs1 rs2 ->
+    regset_lessdef (nextinstr_nf rs1) (nextinstr_nf rs2).
+Proof.
+  intros. unfold nextinstr_nf.
+  eapply regset_lessdef_nextinstr; eauto.
+  eapply regset_lessdef_undef_regs; eauto.
+Qed.
+
+Lemma regset_lessdef_ptr : forall rs1 rs2 r b ofs,
+    regset_lessdef rs1 rs2 ->
+    rs1 r = Vptr b ofs ->
+    rs2 r = Vptr b ofs.
+Proof.
+  intros. generalize (H r). intro.
+  inv H1; congruence.
+Qed.
+
+Lemma step_correct :
+  forall s1 t s2, step init_sup ge s1 t s2 ->
+  forall wp s1' (MS : match_states wp s1 s1'),
+  exists s2', step init_sup ge s1' t s2' /\ match_states wp s2 s2'. 
+Proof.
+  induction 1; intros; inv MS.
+  - (* internal steps *)
+    Ltac 
+    Ltac solve_exec_instr := split;
+                             [econstructor; eauto using regset_lessdef_ptr; try econstructor; eauto | econstructor; eauto ].
+    destruct i; inv EXEC; eexists; solve_exec_instr.
+    + eapply regset_lessdef_nextinstr. eapply regset_lessdef_set; eauto.
+    + eapply regset_lessdef_nextinstr_nf. eapply regset_lessdef_set; eauto.
+    + eapply regset_lessdef_nextinstr_nf. eapply regset_lessdef_set; eauto.
+    + eapply regset_lessdef_nextinstr_nf. eapply regset_lessdef_set; eauto.
+    + simpl. admit. (*load*)
+    + admit.
+      eapply regset_lessdef_nextinstr_nf. eapply regset_lessdef_set; eauto.
+      
+    admit.
+  - (* builtin steps *)
+  - eexists; split; econstructor; eauto.
+  - edestruct eval_operation_lessdef as [v' [OP LD]]. 3: eauto.
+    apply regs_lessdef_regs. eauto. eauto. eexists. split.
+    eapply exec_Iop; eauto.
+    econstructor; eauto.
+    eapply set_reg_lessdef; eauto.
+  - edestruct eval_addressing_lessdef as [a' [OP LDa]]. 2: eauto.
+    apply regs_lessdef_regs. eauto.
+    edestruct Mem.loadv_extends as [v' [LD LDv]]; eauto.
+    eexists. split.
+    eapply exec_Iload; eauto.
+    econstructor; eauto.
+    eapply set_reg_lessdef; eauto.
+  - edestruct eval_addressing_lessdef as [a' [OP LDa]]. 2: eauto.
+    apply regs_lessdef_regs. eauto.
+    edestruct Mem.storev_extends as [v' [ST Hm']]; eauto.
+    exploit ext_acci_storev. apply H1. apply ST. eauto. 
+    eexists. split.
+    eapply exec_Istore; eauto.
+    econstructor; eauto. instantiate (1:= Hm'). etransitivity; eauto.
+    etransitivity; eauto.
+  - exploit ros_address_lessdef. eauto. instantiate (1:= ros). fold vf.
+    intro.
+    eexists.
+    split. eapply exec_Icall; eauto. eapply find_funct_lessdef; eauto.
+    econstructor; eauto. constructor; eauto. eapply regs_lessdef_regs. eauto.
+  - exploit ros_address_lessdef. eauto. instantiate (1:= ros). fold vf.
+    intro. exploit Mem.free_parallel_extends; eauto.
+    intros [tm' [FREE Hm']]. exploit ext_acci_free. apply H2. apply FREE.  intro AI.
+    eexists.
+    split. eapply exec_Itailcall; eauto. eapply find_funct_lessdef; eauto.
+    econstructor; eauto. eapply regs_lessdef_regs. eauto. instantiate (1:= Hm').
+    etransitivity; eauto. etransitivity; eauto.
+  - edestruct eval_builtin_args_lessdef as [vargs' [EV ARGSLD]]. apply RLD. eauto. eauto.
+    exploit external_call_mem_extends; eauto. intros (vres' & m'1 & A & B & C & D & E).
+    assert (ACCI: ext_acci (extw m m'0 Hm) (extw m' m'1 C)).
+    econstructor; eauto using external_call_tid, external_call_support.
+    red. intros. eauto using external_call_max_perm.
+    red. intros. eauto using external_call_max_perm.
+    eexists. split. eapply exec_Ibuiltin; eauto. econstructor; eauto.
+    apply set_res_lessdef; eauto. instantiate (1:= C).
+    etransitivity; eauto. etransitivity; eauto.
+  - exploit eval_condition_lessdef. apply regs_lessdef_regs. eauto. eauto. eauto.
+    intro. eexists. split. eapply exec_Icond; eauto. econstructor; eauto.
+  - specialize (RLD arg) as ARGLD. rewrite H0 in ARGLD. inv ARGLD.
+    eexists. split.
+    eapply exec_Ijumptable; eauto. econstructor; eauto.
+  - exploit Mem.free_parallel_extends; eauto. intros [m'1 [FREE Hm1]].
+    exploit ext_acci_free. apply H0. apply FREE. intro.
+    eexists. split. eapply exec_Ireturn; eauto. econstructor; eauto.
+    destruct or;  eauto. instantiate (1:= Hm1). etransitivity; eauto. etransitivity; eauto.
+  - exploit Mem.alloc_extends; eauto. reflexivity. reflexivity.
+    intros [m'1 [ALLOC Hm1]]. exploit ext_acci_alloc. apply H. eauto. intro.
+    eexists. split. eapply exec_function_internal; eauto. eapply find_funct_lessdef; eauto.
+    econstructor; eauto. apply regs_lessdef_init_regs. eauto. instantiate (1:= Hm1).
+    etransitivity; eauto. etransitivity; eauto.
+  - exploit external_call_mem_extends; eauto. intros (vres' & m'1 & A & B & C & D & E).
+    assert (ACCI: ext_acci (extw m m'0 Hm) (extw m' m'1 C)).
+    econstructor; eauto using external_call_tid, external_call_support.
+    red. intros. eauto using external_call_max_perm.
+    red. intros. eauto using external_call_max_perm.
+    eexists. split. eapply exec_function_external; eauto. eapply find_funct_lessdef; eauto.
+    econstructor; eauto. instantiate (1:= C).
+    etransitivity; eauto. etransitivity; eauto.
+  - inv STACKS. eexists. split. eapply exec_return; eauto. econstructor; eauto.
+    apply set_reg_lessdef; eauto.
+Qed.
+      
+Lemma initial_correct:
+  forall q1 q2 st1, GS.match_query c_ext w q1 q2 -> initial_state ge q1 st1 ->
+               exists st2, initial_state ge q2 st2 /\ match_states (get w) st1 st2.
+Proof.
+  intros. destruct H. inv H2. clear Hm1. inv H0. CKLR.uncklr. 
+  eexists. split. econstructor; eauto. eapply find_funct_lessdef; eauto.
+  econstructor; eauto. constructor. instantiate (1:= Hm).
+  constructor; eauto; red; intros; eauto. rewrite <- H4. reflexivity.
+Qed.
+
+Lemma final_correct:
+  forall wp st1 st2 r1, match_states wp st1 st2 -> final_state st1 r1 ->
+                   exists r2 wp', final_state st2 r2 /\ (get w) o-> wp' /\ ext_acci wp wp' /\
+                                                               GS.match_reply (c_ext) (CallconvBig.set w wp') r1 r2.
+Proof.
+  intros. inv H0. inv H. inv STACKS.
+  eexists. exists (extw m m' Hm). split.
+  - constructor.
+  - split. auto. split. auto. constructor; CKLR.uncklr; cbn; auto. constructor.
+Qed.
+
+Lemma external_correct:
+  forall wp st1 st2 q1, match_states wp st1 st2 -> at_external ge st1 q1 ->
+  exists wx q2, at_external ge st2 q2 /\ ext_acci wp (get wx) /\  GS.match_query (c_ext) wx q1 q2 /\ se = se /\
+  forall r1 r2 st1' wp'', (get wx) o-> wp'' -> GS.match_reply (c_ext) (CallconvBig.set w wp'') r1 r2 -> after_external st1 r1 st1' ->
+  exists st2', after_external st2 r2 st2' /\ match_states wp'' st1' st2'.
+Proof.
+  intros wp st1 st2 q1 Hst Hq1. destruct Hq1. inv Hst.
+  exists (extw m m' Hm). eexists. intuition idtac.
+  - econstructor; eauto. eapply find_funct_lessdef; eauto.
+  - constructor; CKLR.uncklr; auto. constructor.
+    destruct vf; cbn in *; congruence.
+  - inv H1. inv H2. inv H4. CKLR.uncklr.
+    exists (Returnstate s' vres2 m2'). split. econstructor; eauto. simpl in H1. inv H1.
+    econstructor; eauto. reflexivity. etransitivity. eauto. simpl in H0. eauto.
+Qed.
+
+End EXT.
+
+Theorem RTL_ext_selfsim prog :
+  GS.forward_simulation (c_ext) (RTL.semantics prog) (RTL.semantics prog).
+Proof.
+  constructor.
+  eapply GS.Forward_simulation.
+  + reflexivity.
+  + intros se1 se2 w Hse Hse1. cbn -[semantics] in *.
+  eapply GS.forward_simulation_step; subst.
+  - destruct 1. CKLR.uncklr. destruct H; cbn; try congruence.
+  - eapply initial_correct; eauto.
+  - eapply final_correct; eauto.
+  - eapply external_correct; eauto.
+  - intros. eapply step_correct; eauto.
+  + auto using well_founded_ltof.
+Qed.
